<?xml version="1.0"?>


<!DOCTYPE rdf:RDF [
    <!ENTITY org "http://www.w3.org/ns/org#" >
    <!ENTITY dct "http://purl.org/dc/terms/" >
    <!ENTITY foaf "http://xmlns.com/foaf/0.1/" >
    <!ENTITY rov "http://www.w3.org/ns/regorg#" >
    <!ENTITY sf "http://www.opengis.net/ont/sf#" >
    <!ENTITY owl "http://www.w3.org/2002/07/owl#" >
    <!ENTITY dc "http://purl.org/dc/elements/1.1/" >
    <!ENTITY vcard "http://www.w3.org/2006/vcard/ns#" >
    <!ENTITY gr "http://purl.org/goodrelations/v1#" >
    <!ENTITY xsd "http://www.w3.org/2001/XMLSchema#" >
    <!ENTITY elod "http://linkedeconomy.org/ontology#" >
    <!ENTITY skos "http://www.w3.org/2004/02/skos/core#" >
    <!ENTITY geo "http://www.opengis.net/ont/geosparql#" >
    <!ENTITY rdfs "http://www.w3.org/2000/01/rdf-schema#" >
    <!ENTITY rdf "http://www.w3.org/1999/02/22-rdf-syntax-ns#" >
    <!ENTITY pc "http://purl.org/procurement/public-contracts#" >
]>


<rdf:RDF xmlns="http://linkedeconomy.org/ontology#"
     xml:base="http://linkedeconomy.org/ontology"
     xmlns:dc="http://purl.org/dc/elements/1.1/"
     xmlns:geo="http://www.opengis.net/ont/geosparql#"
     xmlns:foaf="http://xmlns.com/foaf/0.1/"
     xmlns:sf="http://www.opengis.net/ont/sf#"
     xmlns:org="http://www.w3.org/ns/org#"
     xmlns:rov="http://www.w3.org/ns/regorg#"
     xmlns:vcard="http://www.w3.org/2006/vcard/ns#"
     xmlns:rdfs="http://www.w3.org/2000/01/rdf-schema#"
     xmlns:dct="http://purl.org/dc/terms/"
     xmlns:pc="http://purl.org/procurement/public-contracts#"
     xmlns:owl="http://www.w3.org/2002/07/owl#"
     xmlns:xsd="http://www.w3.org/2001/XMLSchema#"
     xmlns:rdf="http://www.w3.org/1999/02/22-rdf-syntax-ns#"
     xmlns:gr="http://purl.org/goodrelations/v1#"
     xmlns:skos="http://www.w3.org/2004/02/skos/core#"
     xmlns:elod="http://linkedeconomy.org/ontology#">
    <owl:Ontology rdf:about="http://linkedeconomy.org/ontology">
        <rdfs:label xml:lang="en">Pilot3 Ontology</rdfs:label>
        <dct:creator xml:lang="en">Eleftherios Galanos</dct:creator>
        <dct:creator xml:lang="en">Giorgos Vafeiadis</dct:creator>
        <dct:creator xml:lang="en">Islam A. Hassan</dct:creator>
        <owl:versionInfo xml:lang="en">Latest Update: 2016-09-16</owl:versionInfo>
        <dct:creator xml:lang="en">Michalis Vafopoulos</dct:creator>
        <dc:title xml:lang="en">Pilot3 Ontology</dc:title>
    </owl:Ontology>
    


    <!-- 
    ///////////////////////////////////////////////////////////////////////////////////////
    //
    // Annotation properties
    //
    ///////////////////////////////////////////////////////////////////////////////////////
     -->

    


    <!-- http://purl.org/dc/elements/1.1/title -->

    <owl:AnnotationProperty rdf:about="&dc;title"/>
    


    <!-- http://purl.org/dc/terms/creator -->

    <owl:AnnotationProperty rdf:about="&dct;creator"/>
    


    <!-- 
    ///////////////////////////////////////////////////////////////////////////////////////
    //
    // Datatypes
    //
    ///////////////////////////////////////////////////////////////////////////////////////
     -->

    


    <!-- http://purl.org/procurement/public-contracts-datatypes#percentage -->

    <rdfs:Datatype rdf:about="http://purl.org/procurement/public-contracts-datatypes#percentage"/>
    


    <!-- http://www.w3.org/2001/XMLSchema#date -->

    <rdfs:Datatype rdf:about="&xsd;date"/>
    


    <!-- http://www.w3.org/2001/XMLSchema#duration -->

    <rdfs:Datatype rdf:about="&xsd;duration"/>
    


    <!-- http://www.w3.org/2001/XMLSchema#gYear -->

    <rdfs:Datatype rdf:about="&xsd;gYear"/>
    


    <!-- 
    ///////////////////////////////////////////////////////////////////////////////////////
    //
    // Object Properties
    //
    ///////////////////////////////////////////////////////////////////////////////////////
     -->

    


    <!-- http://linkedeconomy.org/ontology#awardConcernsNotice -->

    <owl:ObjectProperty rdf:about="&elod;awardConcernsNotice">
        <rdfs:label xml:lang="en">award concerns notice</rdfs:label>
        <rdfs:comment xml:lang="en">Relates an award notice with a notice.</rdfs:comment>
        <rdfs:range rdf:resource="&pc;Contract"/>
        <rdfs:domain rdf:resource="&pc;Contract"/>
    </owl:ObjectProperty>
    


    <!-- http://linkedeconomy.org/ontology#buyer -->

    <owl:ObjectProperty rdf:about="&elod;buyer">
        <rdf:type rdf:resource="&owl;FunctionalProperty"/>
        <rdfs:label xml:lang="en">Buyer of contract</rdfs:label>
        <rdfs:comment xml:lang="en">Buyer of a service or product from a Seller.</rdfs:comment>
        <rdfs:range rdf:resource="&foaf;Agent"/>
    </owl:ObjectProperty>
    


    <!-- http://linkedeconomy.org/ontology#countryIsoCode -->

    <owl:ObjectProperty rdf:about="&elod;countryIsoCode">
        <rdfs:label xml:lang="en">country iso code</rdfs:label>
        <rdfs:comment xml:lang="en">This property links to a skos:Concept representing a country ISO code.</rdfs:comment>
        <rdfs:range rdf:resource="&skos;Concept"/>
    </owl:ObjectProperty>
    


    <!-- http://linkedeconomy.org/ontology#hasCurrency -->

    <owl:ObjectProperty rdf:about="&elod;hasCurrency">
        <rdfs:label xml:lang="en">has currency</rdfs:label>
        <rdfs:comment xml:lang="en">This property defines the Currency for the prices specified by an instance of the “gr:UnitPriceSpecification”.</rdfs:comment>
        <rdfs:range rdf:resource="&skos;Concept"/>
        <rdfs:domain>
            <owl:Class>
                <owl:unionOf rdf:parseType="Collection">
                    <rdf:Description rdf:about="&elod;Amount"/>
                    <rdf:Description rdf:about="&gr;UnitPriceSpecification"/>
                </owl:unionOf>
            </owl:Class>
        </rdfs:domain>
    </owl:ObjectProperty>
    


    <!-- http://linkedeconomy.org/ontology#hasNutsCode -->

    <owl:ObjectProperty rdf:about="&elod;hasNutsCode">
        <rdfs:label xml:lang="en">Nuts code of public contract</rdfs:label>
        <rdfs:comment xml:lang="en">Specifies nuts code of public contract. Only a predefined ramon:NUTSRegion can be used.</rdfs:comment>
        <rdfs:domain rdf:resource="&pc;Contract"/>
        <rdfs:range rdf:resource="http://rdfdata.eionet.europa.eu/ramon/ontology/NUTSRegion"/>
    </owl:ObjectProperty>
    


    <!-- http://linkedeconomy.org/ontology#seller -->

    <owl:ObjectProperty rdf:about="&elod;seller">
        <rdfs:label xml:lang="en">Seller of contract</rdfs:label>
        <rdfs:comment xml:lang="en">Seller of a service or product to a Buyer.</rdfs:comment>
        <rdfs:range rdf:resource="&foaf;Agent"/>
    </owl:ObjectProperty>
    


    <!-- http://purl.org/procurement/public-contracts#additionalObject -->

    <owl:ObjectProperty rdf:about="&pc;additionalObject">
        <rdfs:label xml:lang="en">Additional object of contract</rdfs:label>
        <rdfs:comment xml:lang="en">CPV (Common Procurement Vocabulary) code describing an additional object of a public contract. Cardinality 0..*</rdfs:comment>
        <rdfs:isDefinedBy rdf:resource="http://purl.org/procurement/public-contracts"/>
        <rdfs:domain rdf:resource="&pc;Contract"/>
        <rdfs:range rdf:resource="&skos;Concept"/>
    </owl:ObjectProperty>
    


    <!-- http://purl.org/procurement/public-contracts#agreedPrice -->

    <owl:ObjectProperty rdf:about="&pc;agreedPrice">
        <rdfs:label xml:lang="en">Agreed Price</rdfs:label>
        <rdfs:comment xml:lang="en">After a tender is awarded a Contract, a price is agreed between the awarded supplier and the contracting authority. This property assigns that price is assigned to the Contract.</rdfs:comment>
        <rdfs:comment xml:lang="en">Property for a price stated on the contract with the supplier. Cardinality 0..1</rdfs:comment>
        <rdfs:range rdf:resource="&gr;UnitPriceSpecification"/>
        <rdfs:domain rdf:resource="&pc;Contract"/>
    </owl:ObjectProperty>
    


    <!-- http://purl.org/procurement/public-contracts#authorityKind -->

    <owl:ObjectProperty rdf:about="&pc;authorityKind">
        <rdf:type rdf:resource="&owl;FunctionalProperty"/>
        <rdfs:label xml:lang="en">Kind of contracting authority</rdfs:label>
        <rdfs:comment xml:lang="en">Property for a kind of a contracting authority. Only a predefined SKOS concept can be used. Cardinality 0..1</rdfs:comment>
        <rdfs:range rdf:resource="&skos;Concept"/>
        <rdfs:domain rdf:resource="&foaf;Agent"/>
    </owl:ObjectProperty>
    


    <!-- http://purl.org/procurement/public-contracts#awardCriteriaCombination -->

    <owl:ObjectProperty rdf:about="&pc;awardCriteriaCombination">
        <rdf:type rdf:resource="&owl;FunctionalProperty"/>
        <rdfs:label xml:lang="en">Criteria combination for tender evaluation.</rdfs:label>
        <rdfs:comment xml:lang="en">Property for criteria combination for tender evaluation. Cardinality 0..1</rdfs:comment>
        <rdfs:isDefinedBy rdf:resource="http://purl.org/procurement/public-contracts"/>
        <rdfs:range rdf:resource="&pc;AwardCriteriaCombination"/>
        <rdfs:domain rdf:resource="&pc;Contract"/>
    </owl:ObjectProperty>
    


    <!-- http://purl.org/procurement/public-contracts#awardCriterion -->

    <owl:ObjectProperty rdf:about="&pc;awardCriterion">
        <rdfs:label xml:lang="de">Vergabekriterien</rdfs:label>
        <rdfs:label xml:lang="en">Criterion for contract award.</rdfs:label>
        <rdfs:label xml:lang="fr">Critères d&apos;attribution</rdfs:label>
        <rdfs:comment xml:lang="en">Property for setting a criterion for tender evaluation. Cardinality 0..*</rdfs:comment>
        <rdfs:isDefinedBy rdf:resource="http://purl.org/procurement/public-contracts"/>
        <rdfs:domain rdf:resource="&pc;AwardCriteriaCombination"/>
        <rdfs:range rdf:resource="&pc;CriterionWeighting"/>
    </owl:ObjectProperty>
    


    <!-- http://purl.org/procurement/public-contracts#estimatedPrice -->

    <owl:ObjectProperty rdf:about="&pc;estimatedPrice">
        <rdf:type rdf:resource="&owl;FunctionalProperty"/>
        <rdfs:label xml:lang="cs">Odhadovaná cena zakázky</rdfs:label>
        <rdfs:label xml:lang="en">Exact estimated price</rdfs:label>
        <rdfs:comment xml:lang="cs">Vlastnost pro odhadovanou cenu verejné zakázky. Muže jít o presne odhadovanou cástku nebo interval. Kardinalita 0..1</rdfs:comment>
        <rdfs:comment xml:lang="en">A public contract has usually an estimated price specified before tenders are received. It may be an exact estimated price or a range comprising minimal and maximal estimated price. In both cases, the price is linked to the contract via this property.</rdfs:comment>
        <rdfs:comment xml:lang="en">Property for estimated price of public contract. It can be an exact estimation or an interval. Cardinality 0..1</rdfs:comment>
        <rdfs:range rdf:resource="&gr;UnitPriceSpecification"/>
        <rdfs:isDefinedBy rdf:resource="http://purl.org/procurement/public-contracts"/>
        <rdfs:domain rdf:resource="&pc;Contract"/>
    </owl:ObjectProperty>
    


    <!-- http://purl.org/procurement/public-contracts#kind -->

    <owl:ObjectProperty rdf:about="&pc;kind">
        <rdf:type rdf:resource="&owl;FunctionalProperty"/>
        <rdfs:label xml:lang="en">Contract kind</rdfs:label>
        <rdfs:comment xml:lang="en">Kind of a public contract specifies a basic focus of the contract on works, supplies or services. Only a predefined SKOS concept can be used.</rdfs:comment>
        <rdfs:domain rdf:resource="&pc;Contract"/>
        <rdfs:range rdf:resource="&skos;Concept"/>
    </owl:ObjectProperty>
    


    <!-- http://purl.org/procurement/public-contracts#mainObject -->

    <owl:ObjectProperty rdf:about="&pc;mainObject">
        <rdf:type rdf:resource="&owl;FunctionalProperty"/>
        <rdfs:label xml:lang="en">Main object of contract</rdfs:label>
        <rdfs:comment xml:lang="en">CPV (Common Procurement Vocabulary) code describing the main object of a public contract. Cardinality 0..1</rdfs:comment>
        <rdfs:isDefinedBy rdf:resource="http://purl.org/procurement/public-contracts"/>
        <rdfs:domain rdf:resource="&pc;Contract"/>
        <rdfs:range rdf:resource="&skos;Concept"/>
    </owl:ObjectProperty>
    


    <!-- http://purl.org/procurement/public-contracts#procedureType -->

    <owl:ObjectProperty rdf:about="&pc;procedureType">
        <rdf:type rdf:resource="&owl;FunctionalProperty"/>
        <rdfs:label xml:lang="en">Procedure type</rdfs:label>
        <rdfs:comment xml:lang="en">Type of procedure of a public contract specifies a procedure which is applied to publish information about the contract and choose a supplier. Only a predefined value can be used. Cardinality 0..1</rdfs:comment>
        <rdfs:domain rdf:resource="&pc;Contract"/>
        <rdfs:range rdf:resource="&skos;Concept"/>
    </owl:ObjectProperty>
    


    <!-- http://purl.org/procurement/public-contracts#weightedCriterion -->

    <owl:ObjectProperty rdf:about="&pc;weightedCriterion">
        <rdf:type rdf:resource="&owl;FunctionalProperty"/>
        <rdfs:label xml:lang="en">Weighted criterion</rdfs:label>
        <rdfs:comment xml:lang="en">Property for attaching criterion that is weighted. Cardinality 0..1</rdfs:comment>
        <rdfs:isDefinedBy rdf:resource="http://purl.org/procurement/public-contracts"/>
        <rdfs:domain rdf:resource="&pc;CriterionWeighting"/>
        <rdfs:range rdf:resource="&skos;Concept"/>
    </owl:ObjectProperty>
    


    <!-- http://www.w3.org/2006/vcard/ns#hasAddress -->

    <owl:ObjectProperty rdf:about="&vcard;hasAddress">
        <rdfs:label xml:lang="en">has address</rdfs:label>
        <rdfs:comment xml:lang="en">To specify the components of the delivery address for the object</rdfs:comment>
        <rdfs:range rdf:resource="&vcard;Address"/>
        <rdfs:domain rdf:resource="&foaf;Agent"/>
    </owl:ObjectProperty>
    


    <!-- 
    ///////////////////////////////////////////////////////////////////////////////////////
    //
    // Data properties
    //
    ///////////////////////////////////////////////////////////////////////////////////////
     -->

    


    <!-- http://linkedeconomy.org/ontology#contractId -->

    <owl:DatatypeProperty rdf:about="&elod;contractId">
        <rdfs:label xml:lang="en">contract id</rdfs:label>
        <rdfs:comment xml:lang="en">The unique id of the contract</rdfs:comment>
        <rdfs:domain rdf:resource="&pc;Contract"/>
        <rdfs:range rdf:resource="&xsd;string"/>
    </owl:DatatypeProperty>
    


    <!-- http://linkedeconomy.org/ontology#documentType -->

    <owl:DatatypeProperty rdf:about="&elod;documentType">
        <rdfs:label xml:lang="en">Document Type</rdfs:label>
        <rdfs:comment xml:lang="en">The type of an Administrative Decision.</rdfs:comment>
        <rdfs:domain rdf:resource="&elod;AdministrativeDecision"/>
        <rdfs:range rdf:resource="&xsd;string"/>
    </owl:DatatypeProperty>
    


    <!-- http://linkedeconomy.org/ontology#documentUrl -->

    <owl:DatatypeProperty rdf:about="&elod;documentUrl">
        <rdfs:label xml:lang="en">Document URL</rdfs:label>
        <rdfs:comment xml:lang="en">The URL address of the PDF file of an Administrative Decision.</rdfs:comment>
        <rdfs:domain rdf:resource="&elod;AdministrativeDecision"/>
        <rdfs:range rdf:resource="&xsd;string"/>
    </owl:DatatypeProperty>
    


    <!-- http://linkedeconomy.org/ontology#financialYear -->

    <owl:DatatypeProperty rdf:about="&elod;financialYear">
        <rdfs:label xml:lang="en">Financial Year</rdfs:label>
        <rdfs:comment xml:lang="en">The financial year of an activity.</rdfs:comment>
        <rdfs:range rdf:resource="&xsd;gYear"/>
    </owl:DatatypeProperty>
    


    <!-- http://linkedeconomy.org/ontology#isMatched -->

    <owl:DatatypeProperty rdf:about="&elod;isMatched">
        <rdfs:label xml:lang="en">Flag for matched Organizations</rdfs:label>
        <rdfs:comment xml:lang="en">Flag which shows if organization is matched or not.</rdfs:comment>
        <rdfs:range rdf:resource="&xsd;boolean"/>
        <rdfs:domain rdf:resource="&foaf;Agent"/>
    </owl:DatatypeProperty>
    


    <!-- http://linkedeconomy.org/ontology#tenderDeadline -->

    <owl:DatatypeProperty rdf:about="&elod;tenderDeadline">
        <rdfs:label xml:lang="en">Time-limit for receipt of tenders or requests to participate</rdfs:label>
        <rdfs:comment xml:lang="en">Property for time limit for receipt of tenders or requests to participate. Cardinality 0..1</rdfs:comment>
        <rdfs:domain rdf:resource="&pc;Contract"/>
        <rdfs:range rdf:resource="&xsd;dateTime"/>
    </owl:DatatypeProperty>
    


    <!-- http://purl.org/dc/terms/issued -->

    <owl:DatatypeProperty rdf:about="&dct;issued">
        <rdfs:label xml:lang="en">issued</rdfs:label>
        <rdfs:comment xml:lang="en">Date of formal issuance (e.g., publication) of the resource.</rdfs:comment>
        <rdfs:range rdf:resource="&xsd;dateTime"/>
    </owl:DatatypeProperty>
    


    <!-- http://purl.org/dc/terms/title -->

    <owl:DatatypeProperty rdf:about="&dct;title">
        <rdfs:label xml:lang="en">title</rdfs:label>
        <rdfs:comment xml:lang="en">A name given to the resource.</rdfs:comment>
        <rdfs:range rdf:resource="&xsd;string"/>
    </owl:DatatypeProperty>
    


    <!-- http://purl.org/goodrelations/v1#hasCurrencyValue -->

    <owl:DatatypeProperty rdf:about="&gr;hasCurrencyValue">
        <rdfs:label xml:lang="en">has currency value</rdfs:label>
        <rdfs:comment xml:lang="en">The amount of money specified for a budget or a payment or a public service or a product.</rdfs:comment>
        <rdfs:domain rdf:resource="&elod;Amount"/>
        <rdfs:domain rdf:resource="&gr;UnitPriceSpecification"/>
        <rdfs:range rdf:resource="&xsd;float"/>
    </owl:DatatypeProperty>
    


    <!-- http://purl.org/goodrelations/v1#valueAddedTaxIncluded -->

    <owl:DatatypeProperty rdf:about="&gr;valueAddedTaxIncluded">
        <rdfs:label xml:lang="en">value added tax included</rdfs:label>
        <rdfs:comment xml:lang="en">Indicates whether the VAT is included in the price specified in the decision or not.</rdfs:comment>
        <rdfs:domain rdf:resource="&gr;UnitPriceSpecification"/>
        <rdfs:range rdf:resource="&xsd;boolean"/>
    </owl:DatatypeProperty>
    


    <!-- http://purl.org/procurement/public-contracts#awardDate -->

    <owl:DatatypeProperty rdf:about="&pc;awardDate">
        <rdf:type rdf:resource="&owl;FunctionalProperty"/>
        <rdfs:label xml:lang="en">Date of contract award</rdfs:label>
        <rdfs:comment xml:lang="en">Property for date of contract award to a bidder. Cardinality 0..1</rdfs:comment>
        <rdfs:isDefinedBy rdf:resource="http://purl.org/procurement/public-contracts"/>
        <rdfs:domain rdf:resource="&pc;Contract"/>
        <rdfs:range rdf:resource="&xsd;date"/>
    </owl:DatatypeProperty>
    


    <!-- http://purl.org/procurement/public-contracts#criterionWeight -->

    <owl:DatatypeProperty rdf:about="&pc;criterionWeight">
        <rdfs:label xml:lang="en">Contract award criterion weight</rdfs:label>
        <rdfs:comment xml:lang="en">Property for criterion weight for tender evaluation. Cardinality 0..1</rdfs:comment>
        <rdfs:domain rdf:resource="&pc;CriterionWeighting"/>
        <rdfs:range rdf:resource="http://purl.org/procurement/public-contracts-datatypes#percentage"/>
    </owl:DatatypeProperty>
    


    <!-- http://purl.org/procurement/public-contracts#duration -->

    <owl:DatatypeProperty rdf:about="&pc;duration">
        <rdfs:label xml:lang="en">Duration of contract</rdfs:label>
        <rdfs:comment xml:lang="en">Property for duration of contract. The duration may be described in days, months, years, etc. Cardinality 0..1</rdfs:comment>
        <rdfs:domain rdf:resource="&pc;Contract"/>
        <rdfs:range rdf:resource="&xsd;duration"/>
    </owl:DatatypeProperty>
    


    <!-- http://purl.org/procurement/public-contracts#estimatedEndDate -->

    <owl:DatatypeProperty rdf:about="&pc;estimatedEndDate">
        <rdfs:label xml:lang="en">Estimated end date of contract</rdfs:label>
        <rdfs:comment xml:lang="en">Property for estimated end date of public contract realization. Cardinality 0..1</rdfs:comment>
        <rdfs:domain rdf:resource="&pc;Contract"/>
        <rdfs:range rdf:resource="&xsd;date"/>
    </owl:DatatypeProperty>
    


    <!-- http://purl.org/procurement/public-contracts#startDate -->

    <owl:DatatypeProperty rdf:about="&pc;startDate">
        <rdfs:label xml:lang="en">Start date of contract</rdfs:label>
        <rdfs:comment xml:lang="en">Property for start date of public contract realization coming from the contract&apos;s text.</rdfs:comment>
        <rdfs:domain rdf:resource="&pc;Contract"/>
        <rdfs:range rdf:resource="&xsd;date"/>
    </owl:DatatypeProperty>
    


    <!-- http://www.w3.org/2004/02/skos/core#prefLabel -->

    <owl:DatatypeProperty rdf:about="&skos;prefLabel">
        <rdfs:label xml:lang="en">preferred label</rdfs:label>
        <rdfs:comment xml:lang="en">The Simple Knowledge Organization System provides some basic vocabulary for associating lexical labels with resources of any type. The preferred labels are useful when generating or creating human-readable representations of a knowledge organization system. These labels provide the strongest clues as to the meaning of a SKOS concept.</rdfs:comment>
    </owl:DatatypeProperty>
    


    <!-- http://www.w3.org/2006/vcard/ns#locality -->

    <owl:DatatypeProperty rdf:about="&vcard;locality">
        <rdfs:label xml:lang="en">locality</rdfs:label>
        <rdfs:comment xml:lang="en">The locality (e.g. city or town) associated with the address of the object.</rdfs:comment>
        <rdfs:range rdf:resource="&xsd;string"/>
        <rdfs:domain rdf:resource="&vcard;Address"/>
    </owl:DatatypeProperty>
    


    <!-- http://www.w3.org/2006/vcard/ns#postal-code -->

    <owl:DatatypeProperty rdf:about="&vcard;postal-code">
        <rdfs:label xml:lang="en">postal code</rdfs:label>
        <rdfs:comment xml:lang="en">The postal code associated with the address of the object.</rdfs:comment>
        <rdfs:range rdf:resource="&xsd;string"/>
        <rdfs:domain rdf:resource="&vcard;Address"/>
    </owl:DatatypeProperty>
    


    <!-- http://www.w3.org/2006/vcard/ns#street-address -->

    <owl:DatatypeProperty rdf:about="&vcard;street-address">
        <rdfs:label xml:lang="en">street address</rdfs:label>
        <rdfs:comment xml:lang="en">The street address associated with the address of the object.</rdfs:comment>
        <rdfs:range rdf:resource="&xsd;string"/>
        <rdfs:domain rdf:resource="&vcard;Address"/>
    </owl:DatatypeProperty>
    


    <!-- http://xmlns.com/foaf/0.1/name -->

    <owl:DatatypeProperty rdf:about="&foaf;name">
        <rdfs:label xml:lang="en">name</rdfs:label>
        <rdfs:comment xml:lang="en">A short text describing the respective resource.</rdfs:comment>
        <rdfs:range rdf:resource="&rdfs;Literal"/>
        <rdfs:domain rdf:resource="&foaf;Agent"/>
    </owl:DatatypeProperty>
    


    <!-- 
    ///////////////////////////////////////////////////////////////////////////////////////
    //
    // Classes
    //
    ///////////////////////////////////////////////////////////////////////////////////////
     -->

    


    <!-- http://linkedeconomy.org/ontology#AdministrativeDecision -->

    <owl:Class rdf:about="&elod;AdministrativeDecision">
        <rdfs:label xml:lang="el">Διοικητική απόφαση</rdfs:label>
        <rdfs:label xml:lang="en">Administrative Decision</rdfs:label>
        <rdfs:comment xml:lang="en">Administrative decisions taken by an Organization (Financial &amp; Non Financial).</rdfs:comment>
    </owl:Class>
    


    <!-- http://linkedeconomy.org/ontology#Amount -->

    <owl:Class rdf:about="&elod;Amount">
        <dc:title xml:lang="en">Amount</dc:title>
    </owl:Class>
    


    <!-- http://linkedeconomy.org/ontology#FinancialDecision -->

    <owl:Class rdf:about="&elod;FinancialDecision">
        <rdfs:label xml:lang="el">Οικονομικού Τύπου</rdfs:label>
        <rdfs:label xml:lang="en">Financial Decision</rdfs:label>
        <rdfs:subClassOf rdf:resource="&elod;AdministrativeDecision"/>
        <rdfs:comment xml:lang="en">Financial Decisions are Administrative decisions that involve financial flows (elod:amount).</rdfs:comment>
    </owl:Class>
    


    <!-- http://purl.org/goodrelations/v1#BusinessEntity -->

    <owl:Class rdf:about="&gr;BusinessEntity">
        <rdfs:label xml:lang="en">Business Entity</rdfs:label>
        <rdfs:subClassOf rdf:resource="&foaf;Agent"/>
        <rdfs:comment xml:lang="en">An instance of this class represents the legal agent making (or seeking) a particular offering.</rdfs:comment>
    </owl:Class>
    


    <!-- http://purl.org/goodrelations/v1#UnitPriceSpecification -->

    <owl:Class rdf:about="&gr;UnitPriceSpecification">
        <rdfs:label xml:lang="en">Unit Price Specification</rdfs:label>
        <rdfs:comment xml:lang="en">A conceptual entity that specifies the price asked for a service or product. It specifies the price, the currency and whether the price includes VAT or not.</rdfs:comment>
    </owl:Class>
    


    <!-- http://purl.org/procurement/public-contracts#AwardCriteriaCombination -->

    <owl:Class rdf:about="&pc;AwardCriteriaCombination">
        <rdfs:label xml:lang="cs">Kombinace kritérií pro hodnocení dodaných nabídek</rdfs:label>
        <rdfs:label xml:lang="en">Combination of contract award criteria</rdfs:label>
        <rdfs:comment xml:lang="cs">Trída pro popis kombinace kritérií pro posuzování nabídek zájemcu o zakázku</rdfs:comment>
        <rdfs:comment xml:lang="en">Class for description of criteria combination used for tender evaluation</rdfs:comment>
        <rdfs:isDefinedBy rdf:resource="http://purl.org/procurement/public-contracts"/>
    </owl:Class>
    


    <!-- http://purl.org/procurement/public-contracts#Contract -->

    <owl:Class rdf:about="&pc;Contract">
        <rdfs:label xml:lang="cs">Verejná zakázka</rdfs:label>
        <rdfs:label xml:lang="en">Public contract</rdfs:label>
        <rdfs:subClassOf rdf:resource="&elod;FinancialDecision"/>
        <rdfs:comment xml:lang="cs">Instance této trídy je abstraktní informacní entitou o verejné zakázce. Obsahuje všechny aktuálne známé informace o zakázce, tj. napr. o zadavateli verejné zakázky, službách ci dodávkách, které ve verejné zakázce nakupuje, a o podmínkách nákupu (termíny, ocekávané ceny, atd.). Dále obsahuje informace o nabídkách od zájemcu o zakázku a o vybrané nabídce. Pokud již byla zakázka realizována, obsahuje i informace o skutecné cene za realizaci apod.</rdfs:comment>
        <rdfs:comment xml:lang="en">An instance of this class is an abstract information entity about a public contract. It consists of all currently known information about a contract, e.g., a contracting authority, services or supplies which shall be purchased, and contract conditions (e.g., important dates, expected price, etc.). It also informs about tenders received from particular bidders and about an accepted tender. If the contract has already been realized it also informs about an actual price of realization, etc.</rdfs:comment>
        <rdfs:isDefinedBy rdf:resource="http://purl.org/procurement/public-contracts"/>
    </owl:Class>
    


    <!-- http://purl.org/procurement/public-contracts#CriterionWeighting -->

    <owl:Class rdf:about="&pc;CriterionWeighting">
        <rdfs:label xml:lang="en">Contract award weighted criterion</rdfs:label>
        <rdfs:comment xml:lang="en">Class for description of one criterion and its weight</rdfs:comment>
        <rdfs:isDefinedBy rdf:resource="http://purl.org/procurement/public-contracts"/>
    </owl:Class>
    


    <!-- http://rdfdata.eionet.europa.eu/ramon/ontology/NUTSRegion -->

    <owl:Class rdf:about="http://rdfdata.eionet.europa.eu/ramon/ontology/NUTSRegion">
        <rdfs:label xml:lang="en">NUTS</rdfs:label>
        <rdfs:comment xml:lang="en">Specifies the NUTS (Nomenclature of Territorial Units for Statistics) classification defined by the Eurostat office of the European Union.</rdfs:comment>
    </owl:Class>
    


    <!-- http://www.w3.org/2004/02/skos/core#Concept -->

    <owl:Class rdf:about="&skos;Concept">
        <rdfs:label xml:lang="en">Concept</rdfs:label>
        <rdfs:comment xml:lang="en">This class represents the units of thought - ideas, meanings, or (categories of) objects and events - which underlie many knowledge organization systems.</rdfs:comment>
    </owl:Class>
    


    <!-- http://www.w3.org/2006/vcard/ns#Address -->

    <owl:Class rdf:about="&vcard;Address">
        <rdfs:label xml:lang="en">Address</rdfs:label>
        <rdfs:comment xml:lang="en">Specify the components of the delivery address for the object.</rdfs:comment>
    </owl:Class>
    


    <!-- http://www.w3.org/ns/org#Organization -->

    <owl:Class rdf:about="&org;Organization">
        <rdfs:label xml:lang="en">Organization</rdfs:label>
        <rdfs:subClassOf rdf:resource="&foaf;Agent"/>
        <rdfs:comment xml:lang="en">Represents a collection of people organized together into a community or other social, commercial or political structure. The group has some common purpose or reason for existence which goes beyond the set of people belonging to it and can act as an Agent. Organizations are often decomposable into hierarchical structures.</rdfs:comment>
    </owl:Class>
    


    <!-- http://www.w3.org/ns/regorg#RegisteredOrganization -->

    <owl:Class rdf:about="&rov;RegisteredOrganization">
        <rdfs:label xml:lang="en">Registered Organization</rdfs:label>
        <rdfs:subClassOf rdf:resource="&foaf;Agent"/>
        <rdfs:comment xml:lang="en">It represents an organization that gains legal entity status by the act of registration cf. org:FormalOrganization that applies to any legal entity, including those created by other legal means.</rdfs:comment>
    </owl:Class>
    


    <!-- http://xmlns.com/foaf/0.1/Agent -->

    <owl:Class rdf:about="&foaf;Agent">
        <rdfs:label xml:lang="en">Agent</rdfs:label>
        <rdfs:comment xml:lang="en">The Agent class is the class of agents, things that do stuff. A well known sub-class is Person, representing people. Other kinds of agents include Organization and Group.</rdfs:comment>
    </owl:Class>
    


    <!-- http://xmlns.com/foaf/0.1/Organization -->

    <owl:Class rdf:about="&foaf;Organization">
        <rdfs:label xml:lang="en">Organization</rdfs:label>
        <rdfs:subClassOf rdf:resource="&foaf;Agent"/>
        <rdfs:comment xml:lang="en">Represents a kind of Agent corresponding to social institutions such as companies, societies etc.</rdfs:comment>
    </owl:Class>
</rdf:RDF>



<!-- Generated by the OWL API (version 3.4.2) http://owlapi.sourceforge.net -->

